tuned

formalization/evaluation/prpu-SML/Prpu_Export.sml
@@ -121,19 +121,19 @@ fun shrink (aref, sz) = case aref of
 structure IsabelleMapping = struct
 type 'a ArrayType = 'a array;
 
-fun new_array (a:'a) (n:IntInf.int) = array (IntInf.toInt n, a);
+fun new_array (a:'a) (n:int) = array (n, a);
 
-fun array_length (a:'a ArrayType) = IntInf.fromInt (length a);
+fun array_length (a:'a ArrayType) = length a;
 
-fun array_get (a:'a ArrayType) (i:IntInf.int) = sub (a, IntInf.toInt i);
+fun array_get (a:'a ArrayType) (i:int) = sub (a, i);
 
-fun array_set (a:'a ArrayType) (i:IntInf.int) (e:'a) = update (a, IntInf.toInt i, e);
+fun array_set (a:'a ArrayType) (i:int) (e:'a) = update (a, i, e);
 
 fun array_of_list (xs:'a list) = fromList xs;
 
-fun array_grow (a:'a ArrayType) (i:IntInf.int) (x:'a) = grow (a, IntInf.toInt i, x);
+fun array_grow (a:'a ArrayType) (i:int) (x:'a) = grow (a, i, x);
 
-fun array_shrink (a:'a ArrayType) (sz:IntInf.int) = shrink (a,IntInf.toInt sz);
+fun array_shrink (a:'a ArrayType) (sz:int) = shrink (a,sz);
 
 end;
 
@@ -224,25 +224,25 @@ structure FArray = struct
 structure IsabelleMapping = struct
 type 'a ArrayType = 'a array;
 
-fun new_array (a:'a) (n:IntInf.int) = array (IntInf.toInt n, a);
+fun new_array (a:'a) (n:int) = array (n, a);
 
-fun array_length (a:'a ArrayType) = IntInf.fromInt (length a);
+fun array_length (a:'a ArrayType) = length a;
 
-fun array_get (a:'a ArrayType) (i:IntInf.int) = sub (a, IntInf.toInt i);
+fun array_get (a:'a ArrayType) (i:int) = sub (a, i);
 
-fun array_set (a:'a ArrayType) (i:IntInf.int) (e:'a) = update (a, IntInf.toInt i, e);
+fun array_set (a:'a ArrayType) (i:int) (e:'a) = update (a, i, e);
 
 fun array_of_list (xs:'a list) = fromList xs;
 
-fun array_grow (a:'a ArrayType) (i:IntInf.int) (x:'a) = grow (a, IntInf.toInt i, x);
+fun array_grow (a:'a ArrayType) (i:int) (x:'a) = grow (a, i, x);
 
-fun array_shrink (a:'a ArrayType) (sz:IntInf.int) = shrink (a,IntInf.toInt sz);
+fun array_shrink (a:'a ArrayType) (sz:int) = shrink (a,sz);
 
-fun array_get_oo (d:'a) (a:'a ArrayType) (i:IntInf.int) =
-  sub (a,IntInf.toInt i) handle Subscript => d
+fun array_get_oo (d:'a) (a:'a ArrayType) (i:int) =
+  sub (a,i) handle Subscript => d
 
-fun array_set_oo (d:(unit->'a ArrayType)) (a:'a ArrayType) (i:IntInf.int) (e:'a) =
-  update (a, IntInf.toInt i, e) handle Subscript => d ()
+fun array_set_oo (d:(unit->'a ArrayType)) (a:'a ArrayType) (i:int) (e:'a) =
+  update (a, i, e) handle Subscript => d ()
 
 end;
 end;
@@ -251,16 +251,15 @@ end;
 
 
 
-    fun array_blit src si dst di len = (
-      src=dst andalso raise Fail ("array_blit: Same arrays");
+    fun array_blit src si dst di len = 
       ArraySlice.copy {
-        di = IntInf.toInt di,
-        src = ArraySlice.slice (src,IntInf.toInt si,SOME (IntInf.toInt len)),
-        dst = dst})
+        di=di,
+        src = ArraySlice.slice (src,si,SOME len),
+        dst=dst}
 
-    fun array_nth_oo v a i () = Array.sub(a,IntInf.toInt i) handle Subscript => v | Overflow => v
+    fun array_nth_oo v a i () = Array.sub(a,i) handle Subscript => v
     fun array_upd_oo f i x a () = 
-      (Array.update(a,IntInf.toInt i,x); a) handle Subscript => f () | Overflow => f ()
+      (Array.update(a,i,x); a) handle Subscript => f ()
 
     
 
@@ -1835,19 +1834,16 @@ fun fold f (x :: xs) s = fold f xs (f x s)
 
 fun rev xs = fold (fn a => fn b => a :: b) xs [];
 
-fun new A_ =
-  (fn a => fn b => (fn () => Array.array (IntInf.toInt a, b))) o integer_of_nat;
+fun new A_ = (fn a => fn b => (fn () => Array.array (a, b))) o integer_of_nat;
 
-fun nth A_ a n = (fn () => Array.sub (a, IntInf.toInt (integer_of_nat n)));
+fun nth A_ a n = (fn () => Array.sub (a, integer_of_nat n));
 
 fun upd A_ i x a =
-  (fn () =>
-    let
-      val _ =
-        (fn () => Array.update (a, IntInf.toInt (integer_of_nat i), x)) ();
-    in
-      a
-    end);
+  (fn () => let
+              val _ = (fn () => Array.update (a, integer_of_nat i, x)) ();
+            in
+              a
+            end);
 
 fun map f [] = []
   | map f (x21 :: x22) = f x21 :: map f x22;
@@ -1855,8 +1851,7 @@ fun map f [] = []
 fun image f (Set xs) = Set (map f xs);
 
 fun make A_ n f =
-  (fn () => Array.tabulate (IntInf.toInt (integer_of_nat n),
-    (f o nat_of_integer) o IntInf.fromInt));
+  (fn () => Array.tabulate (integer_of_nat n, f o nat_of_integer));
 
 fun map_of A_ ((l, v) :: ps) k = (if eq A_ l k then SOME v else map_of A_ ps k)
   | map_of A_ [] k = NONE;
