formalization/Prpu_Maxflow/Fifo_Push_Relabel.thy
@@ -1,7 +1,7 @@
 section \<open>FIFO Push Relabel Algorithm\<close>
 theory Fifo_Push_Relabel
 imports 
-  "../Lib/Refine_Add_Fofu"
+  "../Flow_Networks/Lib/Refine_Add_Fofu"
   Generic_Push_Relabel 
 begin
 text \<open>The FIFO push-relabel algorithm maintains a first-in-first-out queue
