formalization/mk_afp_submission.sh
@@ -1,0 +1,64 @@
+#!/bin/bash
+
+DIRS="Flow_Networks Prpu_Maxflow"
+ARCHIVE_NAME="afp-submission.tgz"
+AFP="$HOME/devel/isabelle/afp-2016-1-orig"
+SESSIONS="Prpu_Maxflow"
+
+EXCLUDE="Prpu_Maxflow/Prpu_Benchmark_Export.thy"
+
+
+set -e
+OLDDIR="$PWD"
+TMPDIR=`mktemp -d`
+echo "Preparing submission in $TMPDIR"
+
+TGZ_FILE="$OLDDIR/$ARCHIVE_NAME"
+
+# Collect files
+cp -a $DIRS "$TMPDIR"
+
+cd "$TMPDIR"
+
+# Clean up
+find . -type d -name obsolete | xargs rm -rf
+find . -type d -name output | xargs rm -rf
+find . -name '*~' | xargs rm -rf
+
+find . -name 'NOTGZ' | xargs rm -rf
+find . -name '.gitignore'  | xargs rm -rf
+
+rm -rf $EXCLUDE
+
+# Ughly post-processing
+find . -name "ROOT" | xargs sed -i -e '/^ *(\*No-AFP/d'
+find . -mindepth 2 -maxdepth 2 -name "*.thy" -or -name "ROOT" | xargs sed -i -e 's|"\$AFP|"..|g'
+find . -mindepth 3 -maxdepth 3 -name "*.thy" -or -name "ROOT" | xargs sed -i -e 's|"\$AFP|"../..|g'
+
+# Make tarfile
+tar -czf "$TGZ_FILE" $DIRS
+
+cd "$OLDDIR"
+
+# Remove temporary dir
+rm -rf "$TMPDIR"
+
+# Setup test
+mkdir "$TMPDIR"
+cd "$TMPDIR"
+
+# Prepare AFP environment
+find "$AFP/thys" -mindepth 1 -maxdepth 1 -type d | xargs -n1 ln -s
+cp -a "$AFP/thys/ROOTS" .
+
+# Extract files
+tar -xzf "$TGZ_FILE"
+
+# Add new folders to ROOTS
+for d in $DIRS; do echo $d >> ROOTS; done
+
+# Test build
+isabelle build -d. $SESSIONS
+
+cd $OLDDIR
+# rm -rf $TMPDIR
